Rename the source-to-source compiler

compiler/backend/source_to_sourceScript.sml
@@ -9,8 +9,8 @@ val _ = new_theory "source_to_source";
 
 val _ = set_grammar_ancestry ["source_let", "misc"];
 
-Definition compile_prog_def:
-  compile_prog = source_let$compile_decs
+Definition compile_def:
+  compile = source_let$compile_decs
 End
 
 val _ = export_theory ();
