compiler/backend/proofs/source_to_sourceProofScript.sml
@@ -16,9 +16,9 @@ val _ = set_grammar_ancestry [
 Theorem compile_semantics:
   ¬semantics_prog s env prog Fail ∧
   semantics_prog s env prog outcome ⇒
-    semantics_prog s env (compile_prog prog) outcome
+    semantics_prog s env (compile prog) outcome
 Proof
-  rw [compile_prog_def]
+  rw [compile_def]
   \\ irule source_letProofTheory.compile_semantics
   \\ gs []
 QED
